src/tls/Negotiation.fst
@@ -176,6 +176,11 @@ let find_quic_parameters o: option TLSConstants.quicParameters =
   | Some (Extensions.E_quic_parameters qp) -> Some qp
   | _ -> None
 
+let find_cookie o =
+  match find_client_extension Extensions.E_cookie? o with
+  | None -> None
+  | Some (Extensions.E_cookie c) -> Some c
+
 // finding the pre-shared keys in ClientHello
 let find_pske o =
   match find_client_extension Extensions.E_pre_shared_key? o with
@@ -273,7 +278,7 @@ noeq type mode =
     // more from SH (both TLS 1.2 and TLS 1.3)
     n_protocol_version: protocolVersion ->
     n_server_random: TLSInfo.random ->
-    n_sessionID: option sessionID {n_sessionID = None <==> n_protocol_version = TLS_1p3} ->
+    n_sessionID: sessionID ->
     n_cipher_suite: cipherSuite ->
 
     // redundant with the server extension response?
@@ -304,19 +309,13 @@ let find_server_quic_parameters m =
   | Some (Extensions.E_quic_parameters qp) -> Some qp
   | _ -> None
 
-(* this equality check is not compiled currently - jroesch*)
-private let mode_sessionID_eq_ch_sessionID (m : mode) : bool =
-match m.n_sessionID, m.n_offer.ch_sessionID with
-| None, _ -> false
-| (Some id1), id2 -> id1 = id2
-
 let is_resumption12 m =
   not (is_pv_13 m.n_protocol_version)  &&
-  mode_sessionID_eq_ch_sessionID m
- 
+  m.n_sessionID = m.n_offer.ch_sessionID
+
 let is_cacheable12 m =
   not (is_pv_13 m.n_protocol_version)  &&
-  ( let Some sid = m.n_sessionID in
+  ( let sid = m.n_sessionID in
     sid <> m.n_offer.ch_sessionID &&
     sid <> empty_bytes)
 
@@ -426,7 +425,7 @@ let computeOffer r cfg resume nonce ks pskinfo =
     | _ -> false in
   let qp =
     match cfg.quic_parameters with
-    | Some (qv::_, qp) -> Some (QuicParametersClient qv qv qp)
+    | Some (qv::_, qp) -> Some (QuicParametersClient qv qp)
     | _ -> None in
   let extensions =
     Extensions.prepareExtensions
@@ -541,8 +540,7 @@ let resume_12 mode =
   is_pv_13 mode.n_protocol_version &&
   Some? (find_sessionTicket mode.n_offer) &&
   length mode.n_offer.ch_sessionID > 0 &&
-  Some? mode.n_sessionID &&
-  Some?.v mode.n_sessionID = mode.n_offer.ch_sessionID
+  mode.n_sessionID = mode.n_offer.ch_sessionID
 
 val local_config: #region:rgn -> #role:TLSConstants.role -> t region role -> config
 let local_config #region #role ns =
@@ -589,6 +587,14 @@ let version #region #role ns =
   | S_ClientHello mode _
   | S_Mode mode _
   | S_Complete mode _ -> mode.n_protocol_version
+
+(** Returns cfg.max_versionsion or the negotiated version, when known *)
+val is_hrr: #region:rgn -> #role:TLSConstants.role -> t region role ->
+  ST bool
+  (requires (fun _ -> True))
+  (ensures (fun h0 _ h1 -> h0 == h1))
+let is_hrr #region #role ns =
+  C_HRR? (!ns.state)
 
 (*
 val getSigningKey: #a:Signature.alg -> #region:rgn -> #role:TLSConstants.role -> t region role ->
@@ -655,48 +661,50 @@ let group_of_hrr hrr : option CommonDH.group =
     CommonDH.group_of_namedGroup ng
   | _ -> None
 
-private let choose_extension (kse: CommonDH.keyShareEntry)
-                             (e:Extensions.extension) =
-       if Extensions.E_key_share? e
-       then Some (Extensions.E_key_share (CommonDH.ClientKeyShare [kse]))
-       else if Extensions.E_early_data? e 
-       then None
-       else Some e // TODO filter PSK
-
-let client_HelloRetryRequest #region (ns:t region Client) hrr (s:share) =
-  let { hrr_protocol_version = pv;
+private 
+let choose_extension (s:option share)
+                     (e:Extensions.extension) =
+      match e with
+      | Extensions.E_key_share (CommonDH.ClientKeyShare sl) ->
+        (match s with
+         | Some (| g, gx |) ->
+           Some (Extensions.E_key_share (CommonDH.ClientKeyShare [CommonDH.Share g gx]))
+         | _ -> Some e)
+      | Extensions.E_early_data _ ->
+        None
+      | e -> Some e
+      
+let client_HelloRetryRequest #region (ns:t region Client) hrr (s:option share) =
+  let { hrr_sessionID = sid;
         hrr_cipher_suite = cs;
         hrr_extensions = el } = hrr in
-  match HST.op_Bang ns.state with
+  trace ("Got HRR, extensions: ["^(Extensions.string_of_extensions el)^"]");
+  match ! ns.state with
   | C_Offer offer ->
     let old_shares = gs_of offer in
     let old_psk =
       match find_pske offer with
       | None -> []
       | Some pskl -> pskl in
-    let (| g, gx |) = s in
+    // TODO early data not recorded in retryInfo
+    let ext' = TLSConstants.choose_aux s choose_extension (Some?.v offer.ch_extensions) in
 
-    (match group_of_hrr hrr, find_supported_groups offer with
-    | Some g', Some ngl ->
-      if g = g' && List.Tot.mem (Some?.v (CommonDH.namedGroup_of_group g')) ngl then
-       begin
-        // TODO early data not recorded in retryInfo
-        let ext' = TLSConstants.choose_aux (CommonDH.Share g gx) choose_extension (Some?.v offer.ch_extensions) in
+    // Echo the cookie for QUIC stateless retry
+    let ext' = match List.Tot.find Extensions.E_cookie? el with
+      | Some cookie -> cookie :: ext'
+      | None -> ext' in
 
-        // Echo the cookie for QUIC stateless retry
-        let ext' = match List.Tot.find Extensions.E_cookie? el with
-          | Some cookie -> cookie :: ext'
-          | None -> ext' in
-
-        let offer' = {offer with ch_extensions = Some ext'} in
-        let ri = (hrr, old_shares, old_psk) in
-        HST.op_Colon_Equals ns.state (C_HRR offer' ri);
-        Correct(offer')
-       end
-      else
-        Error(AD_illegal_parameter, "server asked for an invalid group in HRR")
-    | _ ->
-      Error(AD_illegal_parameter, "only keyShare-based HRR is supported on client"))
+    if sid <> offer.ch_sessionID then
+      Error(AD_illegal_parameter, "mismatched session ID in HelloRetryRequest")
+    else if None? (group_of_hrr hrr) && None? ns.cfg.quic_parameters then
+      Error(AD_illegal_parameter, "only keyShare-based HRR is supported on client")
+    else
+     begin
+      let offer' = {offer with ch_extensions = Some ext'} in
+      let ri = (hrr, old_shares, old_psk) in
+      ns.state := (C_HRR offer' ri);
+      Correct(offer')
+     end
 
 (**
   Checks that the protocol version in ClientHello is
@@ -707,8 +715,10 @@ let client_HelloRetryRequest #region (ns:t region Client) hrr (s:share) =
 // usable on both sides; following https://tlswg.github.io/tls13-spec/#rfc.section.4.2.1
 let offered_versions min_pv (o: offer): result (l: list protocolVersion {l <> []}) =
   match find_supported_versions o with
-  | Some []  -> Error(AD_protocol_version, "protocol version negotiation: empty proposal")
-  | Some vs -> Correct vs  // might check no proposal is below min_pv
+  | Some (ServerPV _)
+  | Some (Extensions.ClientPV []) ->
+    Error(AD_protocol_version, "protocol version negotiation: empty proposal")
+  | Some (ClientPV vs) -> Correct vs  // might check no proposal is below min_pv
   | None -> // use legacy offer
       match o.ch_protocol_version, min_pv with
       | TLS_1p0, TLS_1p0 -> Correct [TLS_1p0]
@@ -889,16 +899,16 @@ let client_ServerHello #region ns sh =
     let ssid = sh.sh_sessionID in
     let cext = offer.ch_extensions in
     let sig  = CoreCrypto.RSASIG in
-    let resume = ssid = Some offer.ch_sessionID && length offer.ch_sessionID > 0 in
+    let resume = ssid = offer.ch_sessionID && length offer.ch_sessionID > 0 in
     trace ("processing server extensions "^string_of_option_extensions sext);
-    if not (acceptableVersion ns.cfg spv sr) then
-      Error(AD_illegal_parameter, perror __SOURCE_FILE__ __LINE__ "Protocol version negotiation")
-    else if not (acceptableCipherSuite ns.cfg spv cs) then
-      Error(AD_illegal_parameter, perror __SOURCE_FILE__ __LINE__ "Ciphersuite negotiation")
-    else
-     match Extensions.negotiateClientExtensions spv ns.cfg cext sext cs None resume with
-      | Error z -> Error z
-      | Correct () ->
+    (match Extensions.negotiateClientExtensions spv ns.cfg cext sext cs None resume with
+    | Error z -> Error z
+    | Correct spv ->
+      if not (acceptableVersion ns.cfg spv sr) then
+        Error(AD_illegal_parameter, perror __SOURCE_FILE__ __LINE__ "Protocol version negotiation")
+      else if not (acceptableCipherSuite ns.cfg spv cs) then
+        Error(AD_illegal_parameter, perror __SOURCE_FILE__ __LINE__ "Ciphersuite negotiation")
+      else (
         trace ("negotiated "^string_of_pv spv^" "^string_of_ciphersuite cs);
         match cs with
         | CipherSuite13 ae ha ->
@@ -927,7 +937,7 @@ let client_ServerHello #region ns sh =
                 None // n_hrr
                 spv
                 sr
-                None // (Some ssid)
+                ssid
                 cs
                 pski
                 sext
@@ -959,7 +969,7 @@ let client_ServerHello #region ns sh =
           in
           HST.op_Colon_Equals ns.state (C_Mode mode);
           Correct mode
-        | _ -> Error (AD_decode_error, "ServerHello ciphersuite is not a real ciphersuite")
+        | _ -> Error (AD_decode_error, "ServerHello ciphersuite is not a real ciphersuite")))
 
 (* ---------------- signature stuff, to be removed from Handshake -------------------- *)
 
@@ -1220,7 +1230,6 @@ irreducible val computeServerMode:
   serverRandom: TLSInfo.random ->
   St (result serverMode)
 let computeServerMode cfg co serverRandom =
-  // for now, we set the version before negotiating the rest; this may lead to mismatches e.g. on tickets or certificates
   match negotiate_version cfg co with
   | Error z -> Error z
   | Correct TLS_1p3 ->
@@ -1233,18 +1242,25 @@ let computeServerMode cfg co serverRandom =
     let scert =
       match find_signature_algorithms co with
       | None -> None
-      | Some sigalgs -> 
-        cert_select_cb cfg (get_sni co) sigalgs
+      | Some sigalgs ->
+        let sigalgs =
+          TLSConstants.filter_aux cfg.signature_algorithms TLSConstants.mem_rev sigalgs
+        in
+        if sigalgs = [] then None
+        else cert_select_cb cfg (get_sni co) sigalgs
       in
     match compute_cs13 cfg co pske shares (Some? scert) with
     | Error z -> Error z
     | Correct ([], None) -> Error(AD_handshake_failure, "ciphersuite negotiation failed")
     | Correct ([], Some (ng, cs)) ->
       let hrr = {
-        hrr_protocol_version = TLS_1p3;
+        hrr_sessionID = co.ch_sessionID;
         hrr_cipher_suite = cs;
-        hrr_extensions = [Extensions.E_key_share (CommonDH.HRRKeyShare ng)]; // TODO cookie
-      } in
+        hrr_extensions = [
+          Extensions.E_supported_versions (Extensions.ServerPV TLS_1p3);
+          Extensions.E_key_share (CommonDH.HRRKeyShare ng);
+          Extensions.E_cookie (CoreCrypto.random 32)
+        ]; } in
       Correct(ServerHelloRetryRequest hrr)
     | Correct ((PSK_EDH j ogx cs)::_, _) ->
       (trace "Negotiated PSK_EDH key exchange";
@@ -1253,7 +1269,7 @@ let computeServerMode cfg co serverRandom =
         None
         TLS_1p3
         serverRandom
-        None
+        co.ch_sessionID
         cs
         (Some j)
         None // Extensions will be filled in next pass
@@ -1274,7 +1290,7 @@ let computeServerMode cfg co serverRandom =
           None
           TLS_1p3
           serverRandom
-          None
+          co.ch_sessionID
           cs
           None // No PSKs, pure (EC)DHE
           None // Extensions will be filled in next pass
@@ -1300,7 +1316,7 @@ let computeServerMode cfg co serverRandom =
         None // TODO: no HRR
         pv
         serverRandom
-        (Some co.ch_sessionID)
+        co.ch_sessionID
         cs
         None
         None // Extensions
@@ -1332,7 +1348,7 @@ let computeServerMode cfg co serverRandom =
                 None // no HRR before TLS 1.3
                 pv
                 serverRandom
-                (Some (CoreCrypto.random 32))
+                (CoreCrypto.random 32)
                 cs
                 None
                 None // Extensions will be filled later
@@ -1354,25 +1370,29 @@ private
 let accum_string_of_pv s pv = s ^ " " ^ string_of_pv pv
 
 private
-let aux_extension_ok (o1, ng) (e:Extensions.extension) =
-     match e with
-     | Extensions.E_key_share (CommonDH.ClientKeyShare ecl) ->
-          (match ecl with
-          | [CommonDH.Share g _] -> CommonDH.namedGroup_of_group g = Some ng
-          | _ -> (IO.debug_print_string "Bad key_share\n") && false)
-     | Extensions.E_early_data _ -> false // Forbidden
-     | Extensions.E_cookie c -> true // FIXME we will send cookie
+let aux_extension_ok (o1, hrr) (e:Extensions.extension) =
+    match e with
+    | Extensions.E_key_share (CommonDH.ClientKeyShare ecl) ->
+          (match ecl, group_of_hrr hrr with
+          | [CommonDH.Share g _], Some g' -> g = g'
+          | _, None ->
+            let shares1 = find_key_shares o1 in
+            Some? shares1 &&
+            CommonDH.clientKeyShareBytes (Some?.v shares1) = CommonDH.clientKeyShareBytes ecl
+          | _ -> false)
+    | Extensions.E_early_data _ -> false // Forbidden
+    | Extensions.E_cookie c -> true // FIXME we will send cookie
         // If we add cookie support we need to treat this case separately
         // | Extensions.E_cookie c -> c = S_HRR?.cookie ns.state
-     | e ->
-         (match find_client_extension_aux e Extensions.sameExt o1 with
+    | e ->
+          (match find_client_extension_aux e Extensions.sameExt o1 with
           | None -> (IO.debug_print_string "Extra extension\n") && false
           // This allows the client to send less extensions,
           // but the ones that are sent must be exactly the same
           | Some e' ->
             //FIXME: Extensions.E_pre_shared_key "may be updated" 4.1.2
             true) // FIXME
-            //equalBytes (extensionBytes e) (extensionBytes e'))
+            //(extensionBytes e) = (extensionBytes e'))
         
 val server_ClientHello: #region:rgn -> t region Server ->
   HandshakeMessages.ch ->
@@ -1384,16 +1404,15 @@ let server_ClientHello #region ns offer =
   match HST.op_Bang ns.state with
   | S_HRR o1 hrr ->
     let o2 = offer in
-    // We only send HRR for KeyShare
-    let [Extensions.E_key_share (CommonDH.HRRKeyShare ng)] = hrr.hrr_extensions in
     if
       o1.ch_protocol_version = o2.ch_protocol_version &&
       o1.ch_client_random = o2.ch_client_random &&
       o1.ch_sessionID = o2.ch_sessionID &&
+      o1.ch_sessionID = hrr.hrr_sessionID &&
       List.Tot.mem hrr.hrr_cipher_suite o2.ch_cipher_suites &&
       o1.ch_compressions = o2.ch_compressions &&
       Some? o2.ch_extensions && Some? o1.ch_extensions &&
-      TLSConstants.forall_aux (o1, ng) aux_extension_ok (Some?.v o2.ch_extensions)
+      TLSConstants.forall_aux (o1, hrr) aux_extension_ok (Some?.v o2.ch_extensions)
     then
       let sm = computeServerMode ns.cfg offer ns.nonce in
       match sm with
@@ -1419,10 +1438,23 @@ let server_ClientHello #region ns offer =
       HST.op_Colon_Equals ns.state (S_HRR offer hrr);
       sm
     | Correct (ServerMode m cert) ->
-      trace ("negotiated "^string_of_pv m.n_protocol_version^" "^string_of_ciphersuite m.n_cipher_suite);
-      HST.op_Colon_Equals ns.state (S_ClientHello m cert);
-      sm
-
+      // Forcing HRR for source address validation
+      if ns.cfg.offer_shares = [] then
+        let hrr = ({
+          hrr_sessionID = offer.ch_sessionID;
+          hrr_cipher_suite = m.n_cipher_suite;
+          hrr_extensions = [
+            Extensions.E_supported_versions (Extensions.ServerPV TLS_1p3);
+            Extensions.E_cookie (CoreCrypto.random 32)
+          ]}) in
+        ns.state := (S_HRR offer hrr);
+        Correct (ServerHelloRetryRequest hrr)
+      else
+       begin
+        trace ("negotiated "^string_of_pv m.n_protocol_version^" "^string_of_ciphersuite m.n_cipher_suite);
+        ns.state := (S_ClientHello m cert);
+        sm
+       end
 
 let share_of_serverKeyShare (ks:CommonDH.serverKeyShare) : share =
   let CommonDH.Share g gy = ks in (| g, gy |)
@@ -1434,17 +1466,17 @@ let server_ServerShare #region ns ks =
   | S_ClientHello mode cert ->
     let cexts = mode.n_offer.ch_extensions in
     trace ("processing client extensions " ^ string_of_option_extensions cexts);
-    let scrut = Extensions.negotiateServerExtensions
-        mode.n_protocol_version
-        cexts
-        mode.n_offer.ch_cipher_suites
-        ns.cfg
-        mode.n_cipher_suite
-        None  // option (TI.cVerifyData*TI.sVerifyData)
-        mode.n_pski
-        (Option.mapTot CommonDH.ServerKeyShare ks)
-        (mode_sessionID_eq_ch_sessionID mode) in
-    match scrut with
+    match Extensions.negotiateServerExtensions
+      mode.n_protocol_version
+      cexts
+      mode.n_offer.ch_cipher_suites
+      ns.cfg
+      mode.n_cipher_suite
+      None  // option (TI.cVerifyData*TI.sVerifyData)
+      mode.n_pski
+      (Option.mapTot CommonDH.ServerKeyShare ks)
+      (mode.n_sessionID = mode.n_offer.ch_sessionID)
+    with
     | Error z -> Error z
     | Correct sexts ->
       begin
