src/tls/Test.CommonDH.fst
@@ -1,0 +1,68 @@
+module Test.CommonDH
+
+open FStar.Bytes
+open FStar.Error
+open FStar.Printf
+open FStar.HyperStack
+open FStar.HyperStack.ST
+
+
+open Parse
+open TLSError
+open TLSConstants
+
+module DH = CommonDH
+
+let prefix = "Test.CommonDH"
+
+val discard: bool -> ST unit
+  (requires (fun _ -> True))
+  (ensures (fun h0 _ h1 -> h0 == h1))
+let discard _ = ()
+let print s = discard (IO.debug_print_string (prefix^": "^s^".\n"))
+// let print = C.String,print
+// let print = FStar.HyperStack.IO.print_string
+
+val test: DH.group -> St bool
+let test group =
+  let initiator_key_and_share = DH.keygen group in
+  let gx = DH.pubshare initiator_key_and_share in
+  let gy, gxy = DH.dh_responder gx in
+  let gxy' = DH.dh_initiator initiator_key_and_share gy in
+  let gxy  = hex_of_bytes gxy in
+  let gxy' = hex_of_bytes gxy' in
+  if gxy = gxy' then true
+  else
+    begin
+      print ("Unexpected output: output = " ^ gxy' ^ "\nexpected = " ^ gxy);
+      false
+    end
+
+let groups : list Parse.namedGroup =
+  let open CoreCrypto in
+  let open Parse in
+  [
+    FFDHE FFDHE2048;
+    FFDHE FFDHE3072;
+    FFDHE FFDHE4096;
+    FFDHE FFDHE6144;
+    FFDHE FFDHE8192;
+    SEC ECC_P256;
+    SEC ECC_P384;
+    SEC ECC_P521;
+    SEC ECC_X25519;
+    // TODO: Not implemented; see ECGroup.fst
+    //SEC ECC_X448
+  ]
+
+let rec test_groups (groups:list Parse.namedGroup) : St bool =
+  match groups with
+  | g :: gs ->
+    let Some group = DH.group_of_namedGroup g in
+    print ("Testing " ^ DH.string_of_group group);
+    test group && test_groups gs
+  | _ -> true
+
+// Called from Test.Main
+let main () =
+  if test_groups groups then C.EXIT_SUCCESS else C.EXIT_FAILURE
