src/tls/concrete-flags/Flags.fst
@@ -5,7 +5,7 @@ inline_for_extraction let debug = false
 inline_for_extraction let debug_QUIC = debug
 inline_for_extraction let debug_CDH = debug
 inline_for_extraction let debug_Epochs = debug
-inline_for_extraction let debug_FFI = debug 
+inline_for_extraction let debug_FFI = debug
 inline_for_extraction let debug_HS = debug
 inline_for_extraction let debug_HSL = debug
 inline_for_extraction let debug_KS = debug
@@ -15,7 +15,7 @@ inline_for_extraction let debug_TLS = debug
 inline_for_extraction let debug_AEP = debug
 
 inline_for_extraction let ideal_KEF = false
-inline_for_extraction let ideal_Nonce = false  
+inline_for_extraction let ideal_Nonce = false
 inline_for_extraction let ideal_Sig = false
 inline_for_extraction let ideal_PMS = false
 inline_for_extraction let ideal_PRF = false
